IsaHipster.thy
@@ -10,9 +10,8 @@ structure Hipster_Setup =
 struct
 
 
-(* FIXME: Default to Isabelle Contrib or something more sensible *)
 (* Set these to your path to the Hipster directory *)
-val basepath = "~/Field/IsaHipster/";
+val basepath = "$HIPSTER_HOME/";
 val filepath = basepath^"GenCode/";
 
 end
